$$
\begin{align*}  
f'(x) &= 7f(x) + 2g(x) \\  
g'(x) &= -4f(x) + g(x)  
\end{align*}
$$

$$
\begin{align*}  
f' &= 7f + 2g \\  
g' &= -4f + g \\
f' &= 7f + 2g \\  
2g' &= -8f + 2g \\
f' - 2g' &= -f \\  
\\
f' &= 7f + 2g \\  
g' &= -4f + g \\
\end{align*}
$$

$$f(t) = c_1 e^{3 t} (2 e^{2 t} - 1) + c_2 e^{3t} (e^{2 t} - 1)$$
$$g(t) = -2 c_1 e^{(3 t)} (e^{(2 t)} - 1) - c_2 e^{(3 t)} (e^{(2 t)} - 2)$$
$$
\begin{align*}  
\frac{d}{dx} \left( 16 e^{5x} - 13 e^{3x} \right)  &= 7(16 e^{5x} - 13 e^{3x}) + 2(26e^{3x}-16e^{5x}) \\
80e^{5x}-39e^{3x} &= \\
g'(x) &= -4f(x) + g(x)  
\end{align*}
$$
