$$
\begin{align*}  
x &= vt \cos \theta, \\  
y &= vt \sin \theta - \frac{1}{2} gt^2,  
\end{align*}
$$
$$
\begin{align*}
v(t) &= vt \sin \theta - \frac{1}{2} gt^2\\
&\dots \\
v'(t) &= v \sin \theta - gt = 0\\
v \sin \theta &= gt\\
\frac{v \sin \theta}{g} &= t\\
\end{align*}
$$

The peak is at $t_{1}=\frac{v\sin \theta}{g}$. This means the second $x$-intercept is at $t_{2} = \frac{2v \sin \theta}{g}$

This means we need a parabola that goes through $(0,0)$, $(u(t_{1}), v(t_{1}))$ and $(u(t_{2}), 0)$.

$$\begin{align}
\left( v \cdot \frac{v\sin \theta}{g} \cdot\cos \theta, v\left( \frac{v\sin \theta}{g} \right)  \sin \theta - \frac{1}{2} g\left( \frac{v\sin \theta}{g} \right) ^2\right) \\
\left(\frac{v^2 \sin \theta \cos \theta}{g}, \frac{v^2\sin^2 \theta}{g} - \frac{1}{2} g\left( \frac{v^2\sin^2 \theta}{g^2} \right)\right) \\
\left(\frac{v^2 \sin \theta \cos \theta}{g}, \frac{v^2\sin^2 \theta}{2g}\right)
\end{align}$$

$$\left(\frac{2v^2 \sin \theta \cos \theta}{g}, 0\right)$$

Converting this parabola to rectangular coordinates...
$$y = -\frac{\frac{v^{2}\sin^{2}\left(\theta\right)}{2g}}{\left( \frac{v^{2}\sin\left(\theta\right)\cos\left(\theta\right)}{g} \right) ^{2}}\left(x-\frac{v^{2}\sin\left(\theta\right)\cos\left(\theta\right)}{g}\right)^{2}+\frac{v^{2}\sin^{2}\left(\theta\right)}{2g}$$
$$y = -\frac{\left(xg-v\sin \left(\theta\right)\cos \left(\theta\right)\right)^2}{2v\cos ^2\left(\theta\right)g}+\frac{v\sin ^2\left(\theta\right)}{2g}$$

$$
\begin{align}
g &= y \\
v &= z\\
\theta&=t
\end{align}$$
